sound -call

GradVerProofs.v
@@ -40,13 +40,20 @@ Ltac emagicProgress :=
   repeat eexists;
   econstructor; econstructor;
   unfold evale; simpl; eauto.
-
+(* 
 Definition soundness : Prop :=
-  forall pre s post initialHeap initialRho initialAccess S',
+  forall pre s post initialHeap initialRho initialAccess,
   hoare pre s post ->
   invAll initialHeap initialRho initialAccess pre ->
   exists finalHeap finalRho finalAccess,
-    dynSemStar (initialHeap, (initialRho, initialAccess, s) :: S') (finalHeap, (finalRho, finalAccess, []) :: S') /\
+    dynSemStar (initialHeap, [(initialRho, initialAccess, s)]) (finalHeap, [(finalRho, finalAccess, [])]) /\
+    invAll finalHeap finalRho finalAccess post.
+ *)
+Definition soundness pre s post initialHeap initialRho initialAccess S : Prop :=
+  hoare pre s post ->
+  invAll initialHeap initialRho initialAccess pre ->
+  exists finalHeap finalRho finalAccess,
+    dynSemStar (initialHeap, (initialRho, initialAccess, s) :: S) (finalHeap, (finalRho, finalAccess, []) :: S) /\
     invAll finalHeap finalRho finalAccess post.
 
 Ltac uninv :=
@@ -82,620 +89,60 @@ Ltac unfoldINV INV :=
 
 Ltac invE H v := inversion H as [v temp]; clear H; rename temp into H.
 
-
-Lemma evale'eSubsts2RhoFrom3 : forall H r z v2 x1 x2 T_r vo1 e,
-  incl (FVe e) [xUserDef z; xthis] ->
-  r x2 = Some v2 ->
-  r x1 = Some (vo vo1) ->
-  evale' H r (eSubsts [(xthis, x1); (xUserDef z, x2)] e) =
-  evale' H (rhoFrom3 xresult (defaultValue T_r) xthis (vo vo1) (xUserDef z) v2) e.
+Lemma dynSemStarNotModifies : forall x ss H1 H2 r1 r2 A1 A2,
+  (∀ s', In s' ss → ¬ writesTo x s') ->
+  dynSemStar
+    (H1, [(r1, A1, ss)])
+    (H2, [(r2, A2, [])]) ->
+  r1 x = r2 x.
 Proof.
-  induction e0; intros; simpl in *.
-  - tauto.
-  - apply inclSingle in H1.
-    unfold xSubsts, rhoFrom3.
-    inversionx H1; simpl.
-    * dec (x_dec (xUserDef z) (xUserDef z)).
-      assumption.
-    * inversionx H4; tauto.
-  - rewrite IHe0; auto.
-Qed.
-
-Lemma footprint'PhiSubsts2RhoFrom3 : forall H r z v2 x1 x2 T_r vo1 a,
-  incl (FV' a) [xUserDef z; xthis] ->
-  r x2 = Some v2 ->
-  r x1 = Some (vo vo1) ->
-  footprint' H r (phi'Substs [(xthis, x1); (xUserDef z, x2)] a) =
-  footprint' H (rhoFrom3 xresult (defaultValue T_r) xthis (vo vo1) (xUserDef z) v2) a.
-Proof.
-  intros.
-  destruct a; simpl in *; try tauto.
-  erewrite evale'eSubsts2RhoFrom3; auto.
-Qed.
-
-Lemma evale'PhiSubsts2RhoFrom3 : forall H r z v2 x1 x2 T_r vo1 e,
-  incl (FVe e) [xUserDef z; xthis] ->
-  r x2 = Some v2 ->
-  r x1 = Some (vo vo1) ->
-  evale' H
-    r
-    (eSubsts [(xthis, x1); (xUserDef z, x2)] e) =
-  evale' H
-    (rhoFrom3 xresult (defaultValue T_r) xthis (vo vo1) (xUserDef z) v2)
-    e.
-Proof.
-  induction e0; intros; simpl in *.
-  - tauto.
-  - unfold xSubsts, rhoFrom3.
-    apply inclSingle in H1.
-    inversionx H1; simpl.
-    * dec (x_dec (xUserDef z) (xUserDef z)).
-      assumption.
-    * inversionx H4; try tauto.
-  - rewrite IHe0; auto.
-Qed.
-
-Lemma inclApp : forall {T : Type} (A1 A2 B : list T),
-  incl (A1 ++ A2) B ->
-  incl A1 B /\ incl A2 B.
-Proof.
-  unfold incl.
-  intros.
-  intuition.
-Qed.
-
-Lemma evalphi'PhiSubsts2RhoFrom3 : forall H r z v2 x1 x2 T_r vo1 a,
-  incl (FV' a) [xUserDef z; xthis] ->
-  r x2 = Some v2 ->
-  r x1 = Some (vo vo1) ->
-  evalphi' H
-    r
-    (footprint' H
-      (rhoFrom3 xresult (defaultValue T_r) xthis (vo vo1) (xUserDef z) v2)
-      a) 
-    (phi'Substs [(xthis, x1); (xUserDef z, x2)] a) ->
-  evalphi' H
-    (rhoFrom3 xresult (defaultValue T_r) xthis (vo vo1) (xUserDef z) v2)
-    (footprint' H
-      (rhoFrom3 xresult (defaultValue T_r) xthis (vo vo1) (xUserDef z) v2)
-      a)
-    a.
-Proof.
-  intros.
-  destruct a; inversionx H4; common; simpl in *.
-  - constructor.
-  - apply inclApp in H1. unf.
-    eca; unfold evale;
-    erewrite evale'eSubsts2RhoFrom3 in *; eauto.
-  - apply inclApp in H1. unf.
-    eca; unfold evale;
-    erewrite evale'eSubsts2RhoFrom3 in *; eauto.
-  - eca; unfold evale;
-    erewrite evale'eSubsts2RhoFrom3 in *; eauto.
-  - apply inclSingle in H1.
-    unfold xSubsts, rhoFrom3 in *.
-    inversionx H1; simpl in *; eca.
-    * dec (x_dec (xUserDef z) xresult). clear de2.
-      dec (x_dec (xUserDef z) xthis). clear de2.
-      dec (x_dec (xUserDef z) (xUserDef z)).
-      rewrite H2 in *. assumption.
-    * inversionx H4; try tauto.
-      dec (x_dec xthis xresult). clear de2.
-      dec (x_dec xthis xthis).
-      rewrite H3 in *. assumption.
+  induction ss; intros; simpl in *.
+  - inversionx H3; try tauto.
+    inversionx H4.
+  - inversionx H3.
+    rename H4 into ds.
+    rename H5 into dss.
+    assert (¬ writesTo x0 a) as wt1. apply H0. tauto.
+    assert (∀ s' : s, In s' ss → ¬ writesTo x0 s') as wt2. intros. apply H0. tauto.
+    inversionx ds; simpl in wt1.
+    * apply IHss in dss; auto.
+    * apply IHss in dss; auto.
+      unfold rhoSubst in dss.
+      dec (x_dec x0 x1); try tauto.
+      contradict wt1.
+      constructor.
+    * apply IHss in dss; auto.
+      unfold rhoSubst in dss.
+      dec (x_dec x0 x1); try tauto.
+      contradict wt1.
+      constructor.
+    * apply IHss in dss; auto.
+      unfold rhoSubst in dss.
+      dec (x_dec x0 xresult); try tauto.
+      contradict wt1.
+      constructor.
+    * admit.
+    * apply IHss in dss; auto.
+    * apply IHss in dss; auto.
+    * apply IHss in dss; auto.
+      unfold rhoSubst in dss.
+      dec (x_dec x0 x1); try tauto.
+      contradict wt1.
+      constructor.
 Admitted.
 
-Lemma evalphiPhiSubsts2RhoFrom3 : forall H r z v2 x1 x2 T_r vo1 p A,
-  incl (FV p) [xUserDef z; xthis] ->
-  r x2 = Some v2 ->
-  r x1 = Some (vo vo1) ->
-  evalphi
-    H
-    r
-    A
-    (phiSubsts2 xthis x1 (xUserDef z) x2 p) ->
-  evalphi
-    H
-    (rhoFrom3 xresult (defaultValue T_r) xthis (vo vo1) (xUserDef z) v2)
-    A 
-    p.
-Proof.
-  induction p0; intros; simpl; try constructor.
-  inversionx H2.
-  simpl in *.
-  inversionx H4.
-  eca.
-  - erewrite footprint'PhiSubsts2RhoFrom3 in H9; eauto.
-    unfold incl. intros.
-    intuition.
-  - apply inclApp in H1. unf.
-    erewrite (footprint'PhiSubsts2RhoFrom3 _ _ _ _ _ _ T_r) in H14; eauto.
-    eapp evalphi'PhiSubsts2RhoFrom3.
-  - apply inclApp in H1. unf.
-    erewrite (footprint'PhiSubsts2RhoFrom3 _ _ _ _ _ _ T_r) in H15; eauto.
-Qed.
+Print soundness.
 
-Lemma disjointAexcept : forall A B,
-  disjoint A B ->
-  Aexcept A B = A.
-Proof.
-  induction A;
-  intros;
-  simpl;
-  try tauto.
-  rewrite cons2app in H0.
-  apply disjointSplitA in H0. unf.
-  apply IHA in H2. rewrite H2.
-  destruct (negb (existsb (A_d'_decb a) B)) eqn: cl; try tauto.
-  apply negb_false_iff in cl.
-  apply existsb_exists in cl. unf.
-  specialize (H1 x0).
-  intuition.
-  contradict H0.
-  constructor.
-  undecb.
-  destruct a, x0. simpl in *.
-  dec (o_dec o0 o1); simpl in *; try discriminate.
-  dec (string_dec f0 f1); simpl in *; try discriminate.
-  tauto.
-Qed.
-
-Lemma evalphiFootprintAccess : ∀ p H r A,
-       evalphi H r A p ->
-       evalphi H r (footprint H r p) p.
-Proof.
-  induction p0; intros; simpl in *; eca.
-  - intuition.
-  - inversionx H1.
-    assumption.
-  - inversionx H1.
-    rewrite AexceptAppFirst.
-    rewrite AexceptSame.
-    simpl.
-    assert (disjoint (footprint H0 r p0) (footprint' H0 r a)).
-      apply evalphiImpliesAccess in H12.
-      unfold incl, disjoint in *.
-      intros.
-      specialize (H12 x0).
-      destruct (classic (In x0 (footprint H0 r p0)));
-      intuition.
-      apply InAexceptNot in H2.
-      intuition.
-    rewrite disjointAexcept; auto.
-    eapp IHp0.
-Qed.
-
-
-Lemma inclAexceptDisjoint : forall A B C,
-  incl A (Aexcept B C) ->
-  disjoint A C.
-Proof.
-  unfold incl, disjoint.
-  intros.
-  specialize (H0 x0).
-  destruct (classic (In x0 A)); intuition.
-  apply InAexceptNot in H2.
-  auto.
-Qed.
-
-Lemma evalphiRemoveAexcept : forall H r p A1 A2,
-  disjoint (footprint H r p) A2 ->
-  evalphi H r A1 p ->
-  evalphi H r (Aexcept A1 A2) p.
-Proof.
-  induction p0; intros; simpl in *; try constructor.
-  inversionx H2.
-  apply disjointSplitA in H1. unf.
-  eca.
-  - unfold incl, disjoint in *.
-    intros.
-    eapp InAexceptConstr.
-    specialize (H2 a0).
-    intuition.
-  - rewrite AexceptComm.
-    eapp IHp0.
-Qed.
-
-Lemma evalphiElemWise : forall H r A1 A2 p,
-  (forall p', In p' p ->
-  (evalphi' H r A1 p' -> evalphi' H r A2 p')
-  ) ->
-  (evalphi  H r A1 p  -> evalphi  H r A2 p ).
-Proof.
-  induction p0;
-  intros; try constructor.
-  inversionx H2.
-  eca.
-  - eapply evalphi'incl in H12; eauto.
-    eapply H1 in H12.
-    * eapp evalphi'ImpliesIncl.
-    * constructor.
-      tauto.
-  - assert (evalphi H0 r A2 p0) as ep.
-    * eapp IHp0.
-      + intros.
-        apply H1 in H3; auto.
-        apply in_cons.
-        auto.
-      + eapp evalphiAexcept.
-    * eapply evalphiImpliesAccess in H13.
-      apply inclAexceptDisjoint in H13.
-      eapp evalphiRemoveAexcept.
-Qed.
-  
-
-Lemma inclxSubsts : forall x0 x1 x2 z x,
-  let xUDz := xUserDef z in
-  In x [xUDz; xthis; xresult] ->
-  In (xSubsts [(xthis, x1); (xUDz, x2); (xresult, x0)] x) [x2; x1; x0].
-Proof.
-    intros.
-    assert (x_decb xUDz xthis = false) as xd1. dec (x_dec xUDz xthis). tauto.
-    assert (x_decb xUDz xresult = false) as xd2. dec (x_dec xUDz xresult). tauto.
-    assert (x_decb xUDz xUDz = true) as xd3. dec (x_dec xUDz xUDz). tauto.
-    unfold xSubsts.
-    inversionx H0; subst; simpl;
-    try rewrite xd3;
-    try tauto.
-    inversionx H1; subst; simpl;
-    try rewrite xd3;
-    try tauto.
-    inversionx H0; subst; simpl;
-    try rewrite xd3;
-    try tauto.
-Qed.
-
-Lemma incleSubsts : forall x0 x1 x2 z e0,
-  let xUDz := xUserDef z in
-  incl (FVe e0) [xUDz; xthis; xresult] ->
-  incl (FVe (eSubsts [(xthis, x1); (xUDz, x2); (xresult, x0)] e0)) [x2; x1; x0].
-Proof.
-  induction e0; intros; simpl in *.
-  - apply inclEmpty.
-  - apply inclSingle.
-    apply inclSingle in H0.
-    eapp inclxSubsts.
-  - eapp IHe0.
-Qed.
-
-Lemma inclPhiSubsts3 : forall x0 x1 x2 z p p',
-  let xUDz := xUserDef z in
-  incl (FV p) [xUDz; xthis; xresult] ->
-  In p' (phiSubsts3 xthis x1 (xUserDef z) x2 xresult x0 p) ->
-  incl (FV' p') [x2; x1; x0].
-Proof.
-  induction p0; intros; simpl in *; inversionx H1;
-  apply inclApp in H0;
-  unf.
-  - destruct a; simpl in *.
-    * apply inclEmpty.
-    * apply inclApp in H1. unf.
-      apply incl_app;
-      eapp incleSubsts.
-    * apply inclApp in H1. unf.
-      apply incl_app;
-      eapp incleSubsts.
-    * eapp incleSubsts.
-    * apply inclSingle.
-      apply inclSingle in H1.
-      eapp inclxSubsts.
-  - eapp IHp0.
-Qed.
-
-
-Lemma incl2PhiSubst3 : 
-  forall fH' iR fR' x0 x1 x2 vo1 v2 vresult z e0,
-  let xUDz := xUserDef z in
-  let fR := rhoSubst x0 vresult iR in
-  incl (FVe e0) [xUDz; xthis; xresult] ->
-  iR x1 = Some (vo vo1) ->
-  iR x2 = Some v2 ->
-  fR' xthis = Some (vo vo1) ->
-  fR' xUDz = Some v2 ->
-  fR' xresult = Some vresult ->
-  x0 <> x2 ->
-  x0 <> x1 ->
-  evale' fH' fR (eSubsts [(xthis, x1); (xUDz, x2); (xresult, x0)] e0) =
-  evale' fH' fR' e0.
-Proof.
-  induction e0; intros; simpl in *.
-  - tauto.
-  - assert (x_decb xUDz xthis = false) as xd1. dec (x_dec xUDz xthis). tauto.
-    assert (x_decb xUDz xresult = false) as xd2. dec (x_dec xUDz xresult). tauto.
-    assert (x_decb xUDz xUDz = true) as xd3. dec (x_dec xUDz xUDz). tauto.
-    apply inclSingle in H0.
-    subst xUDz fR.
-    inversionx H0.
-      rewrite H4.
-      unfold xSubsts, rhoSubst. simpl.
-      rewrite xd3.
-      dec (x_dec x2 x0); tauto.
-    inversionx H8.
-      rewrite H3.
-      unfold xSubsts, rhoSubst. simpl.
-      dec (x_dec x1 x0); tauto.
-    inversionx H0.
-      rewrite H5.
-      unfold xSubsts, rhoSubst. simpl.
-      dec (x_dec x0 x0); tauto.
-    tauto.
-  - subst fR xUDz.
-    erewrite IHe0; eauto.
-Qed.
-
-  (*LHS: xthis, xresult, xUDz
-       --> x1, x0, x2 
-       --> iR x1, vresult, iR x2
-       --> vo1, vresult, v2 *)
-  (*RHS: xthis, xresult, xUDz
-     --> fR' xthis, fR' xresult, fR' xUDz
-     --> r' xthis, vresult, r' xUDz
-     --> vo1, vresult, v2 *)
-
-Lemma evale'2PhiSubsts3 : 
-  forall fH' iR fR' x0 x1 x2 vo1 v2 vresult z e,
-  let xUDz := xUserDef z in
-  let fR := rhoSubst x0 vresult iR in
-  incl (FVe e) [xUDz; xthis; xresult] ->
-  iR x1 = Some (vo vo1) ->
-  iR x2 = Some v2 ->
-  fR' xthis = Some (vo vo1) ->
-  fR' xUDz = Some v2 ->
-  fR' xresult = Some vresult ->
-  x0 <> x2 ->
-  x0 <> x1 ->
-  x1 <> x2 ->
-  evale' fH' fR (eSubsts [(xthis, x1); (xUserDef z, x2); (xresult, x0)] e) =
-  evale' fH' fR' e.
-Proof.
-  induction e0; intros; simpl in *.
-  - tauto.
-  - subst fR.
-    apply inclSingle in H0.
-    unfold xSubsts, rhoSubst. simpl.
-    inversionx H0; subst.
-      dec (x_dec (xUserDef z) xthis). clear de2.
-      dec (x_dec (xUserDef z) (xUserDef z)).
-      rewrite H4.
-      dec (x_dec x2 x0); tauto.
-    inversionx H9; simpl.
-      rewrite H3.
-      dec (x_dec x1 x0); tauto.
-    inversionx H0; simpl.
-      rewrite H5.
-      dec (x_dec x0 x0); tauto.
-    tauto.
-  - subst fR.
-    erewrite IHe0; eauto.
-Qed.
-
-Lemma footprint'2PhiSubsts3 : 
-  forall fH' iR fR' x0 x1 x2 vo1 v2 vresult z p,
-  let xUDz := xUserDef z in
-  let fR := rhoSubst x0 vresult iR in
-  incl (FV' p) [xUDz; xthis; xresult] ->
-  iR x1 = Some (vo vo1) ->
-  iR x2 = Some v2 ->
-  fR' xthis = Some (vo vo1) ->
-  fR' xUDz = Some v2 ->
-  fR' xresult = Some vresult ->
-  x0 <> x2 ->
-  x0 <> x1 ->
-  x1 <> x2 ->
-  footprint' fH' fR (phi'Substs [(xthis, x1); (xUserDef z, x2); (xresult, x0)] p) =
-  footprint' fH' fR' p.
-Proof.
-  intros.
-  destruct p0; simpl in *; try tauto.
-  subst fR.
-  erewrite evale'2PhiSubsts3; eauto.
-Qed.
-
-Lemma footprint2PhiSubsts3 : 
-  forall fH' iR fR' x0 x1 x2 vo1 v2 vresult z p,
-  let xUDz := xUserDef z in
-  let fR := rhoSubst x0 vresult iR in
-  incl (FV p) [xUDz; xthis; xresult] ->
-  iR x1 = Some (vo vo1) ->
-  iR x2 = Some v2 ->
-  fR' xthis = Some (vo vo1) ->
-  fR' xUDz = Some v2 ->
-  fR' xresult = Some vresult ->
-  x0 <> x2 ->
-  x0 <> x1 ->
-  x1 <> x2 ->
-  footprint fH' fR (phiSubsts3 xthis x1 xUDz x2 xresult x0 p) =
-  footprint fH' fR' p.
-Proof.
-  induction p0; intros; simpl in *; try tauto.
-  apply inclApp in H0. unf.
-  subst fR xUDz.
-  rewrite IHp0; auto.
-  erewrite footprint'2PhiSubsts3; eauto.
-Qed.
-
-Lemma AexceptDisjoint : forall A1 A2,
-  disjoint A1 A2 ->
-  Aexcept A1 A2 = A1.
-Proof.
-  unfold disjoint, Aexcept, except.
-  induction A1; intros; simpl in *; try tauto.
-  assert (~ (existsb (A_d'_decb a) A2) = true).
-    intuition.
-    apply existsb_exists in H1.
-    unf.
-    specialize (H0 x0).
-    intuition.
-    undecb.
-    destruct a, x0. simpl in *.
-    dec (o_dec o0 o1); simpl; try discriminate.
-    dec (string_dec f0 f1); simpl; try discriminate.
-    tauto.
-  apply not_true_is_false in H1.
-  rewrite H1. simpl.
-  rewrite IHA1; try tauto.
-  intros.
-  specialize (H0 x0).
-  intuition.
-Qed.
-
-Lemma evalphi2PhiSubsts3 : 
-  forall fH' iR fR' x0 x1 x2 vo1 v2 vresult z ppost fA',
-  let xUDz := xUserDef z in
-  let fR := rhoSubst x0 vresult iR in
-  incl (FV ppost) [xUDz; xthis; xresult] ->
-  iR x1 = Some (vo vo1) ->
-  iR x2 = Some v2 ->
-  fR' xthis = Some (vo vo1) ->
-  fR' xUDz = Some v2 ->
-  fR' xresult = Some vresult ->
-  x0 <> x2 ->
-  x0 <> x1 ->
-  x1 <> x2 ->
-  evalphi
-    fH'
-    fR'
-    fA'
-    ppost ->
-  evalphi
-    fH'
-    fR
-    (footprint fH' fR (phiSubsts3 xthis x1 xUDz x2 xresult x0 ppost))
-    (phiSubsts3 xthis x1 xUDz x2 xresult x0 ppost).
-Proof.
-  induction ppost; intros; simpl in *; try constructor.
-  eca.
-  - intuition.
-  - rename H9 into ep.
-    destruct a;
-    inversion ep as [? | ? ? ? ? ? ? ? ? invc ? inva invb];
-    subst; clear ep invb;
-    simpl in *.
-    * constructor.
-    * apply inclApp in H0. unf.
-      apply inclApp in H9. unf.
-      inversionx inva.
-      eca; unfold evale in *;
-      subst fR xUDz;
-      erewrite incl2PhiSubst3; eauto.
-    * apply inclApp in H0. unf.
-      apply inclApp in H9. unf.
-      inversionx inva.
-      eca; unfold evale in *;
-      subst fR xUDz;
-      erewrite incl2PhiSubst3; eauto.
-    * apply inclApp in H0. unf.
-      inversionx inva.
-      eca; unfold evale in *;
-      subst fR xUDz;
-      erewrite incl2PhiSubst3; eauto.
-    * assert (x_decb xUDz xthis = false) as xd1. dec (x_dec xUDz xthis). tauto.
-      assert (x_decb xUDz xresult = false) as xd2. dec (x_dec xUDz xresult). tauto.
-      assert (x_decb xUDz xUDz = true) as xd3. dec (x_dec xUDz xUDz). tauto.
-      rewrite cons2app in H0.
-      apply inclApp in H0. unf.
-      apply inclSingle in H9.
-      inversionx inva.
-      subst fR. unfold rhoSubst, xSubsts, rhoFrom3 in *. simpl.
-      inversionx H9; subst; simpl.
-        rename H16 into ee.
-        rewrite H4 in ee. inversionx ee.
-        eca. rewrite xd3. dec (x_dec x2 x0); tauto.
-      inversionx H0; subst; simpl.
-        rename H16 into ee.
-        rewrite H3 in ee. simpl in ee. inversionx ee.
-        eca. dec (x_dec x1 x0); tauto.
-      inversionx H9; subst; simpl.
-        rename H16 into ee.
-        rewrite H5 in ee. inversionx ee.
-        eca. dec (x_dec x0 x0); tauto.
-      tauto.
-  - rename H9 into ep.
-    inversion ep as [? | ? ? ? ? ? ? ? ? invc ? inva invb]. subst. clear ep inva invc.
-    assert (disjoint (footprint fH' fR' ppost) (footprint' fH' fR' a)).
-      apply evalphiImpliesAccess in invb.
-      apply inclAexceptDisjoint in invb.
-      apply invb.
-    subst fR xUDz.
-    apply inclApp in H0. unf.
-    erewrite footprint2PhiSubsts3; eauto.
-    erewrite footprint'2PhiSubsts3; eauto.
-    eapply IHppost in invb; eauto.
-    erewrite footprint2PhiSubsts3 in invb; eauto.
-    
-    rewrite AexceptAppFirst.
-    rewrite AexceptSame. simpl.
-    rewrite AexceptDisjoint; auto.
-Qed.
-
-
-Lemma A_sSubstsApp : forall m A1 A2,
-  A_sSubsts m (A1 ++ A2) =
-  A_sSubsts m A1 ++ A_sSubsts m A2.
-Proof.
-  induction A1; intros; try tauto.
-  destruct a.
-  unfold A_sSubsts in *. simpl.
-  rewrite IHA1.
-  tauto.
-Qed.
-
-Lemma A_sSubstsFP' : forall m p,
-  A_sSubsts m (staticFootprint' p) =
-  staticFootprint' (phi'Substs m p).
-Proof.
-  unfold A_sSubsts;
-  destruct p0;
-  tauto.
-Qed.
-
-Lemma sfrmeSubsts : forall x0 x1 x2 z e A,
-  sfrme A e ->
-  sfrme (A_sSubsts [(xthis, x1); (xUserDef z, x2); (xresult, x0)] A) (eSubsts [(xthis, x1); (xUserDef z, x2); (xresult, x0)] e).
-Proof.
-  induction e0; intros; simpl in *; try (constructor; fail).
-  inversionx H0.
-  eapply IHe0 in H5; eauto.
-  eca.
-  unfold A_sSubsts.
-  apply in_flat_map.
-  exists (phiAcc (eSubsts [(xthis, x1); (xUserDef z, x2); (xresult, x0)] e0) f0).
-  split.
-  - unfold phiSubsts, phi'Substs.
-    apply in_map_iff.
-    exists (phiAcc e0 f0).
-    intuition.
-    apply in_map_iff.
-    eex. tauto.
-  - constructor.
-    tauto.
-Qed.
-
-Lemma sfrmphiPhiSubsts3 : forall x0 x1 x2 z p A,
-  sfrmphi A p ->
-  sfrmphi (A_sSubsts [(xthis, x1); (xUserDef z, x2); (xresult, x0)] A) (phiSubsts [(xthis, x1); (xUserDef z, x2); (xresult, x0)] p).
-Proof.
-  induction p0; intros; try tauto.
-  inversionx H0.
-  eapply IHp0 in H2; eauto.
-  eca.
-  - inversionx H1; simpl; eca;
-    eapp sfrmeSubsts.
-  - rewrite A_sSubstsApp in H2.
-    rewrite A_sSubstsFP' in H2.
-    assumption.
-Qed.
-
-Theorem staSemSoundness : forall (s'' : s) (s' : list s) (pre post : phi) initialHeap initialRho initialAccess S',
+Theorem staSemSoundness : forall (s'' : s) (s' : list s) (pre post : phi) initialHeap initialRho initialAccess,
   hoareSingle pre s'' post ->
   invAll initialHeap initialRho initialAccess pre ->
   exists finalHeap finalRho finalAccess,
-    dynSemStar (initialHeap, (initialRho, initialAccess, s'' :: s') :: S') (finalHeap, (finalRho, finalAccess, s') :: S') /\
+    dynSemStar (initialHeap, [(initialRho, initialAccess, s'' :: s')]) (finalHeap, [(finalRho, finalAccess, s')]) /\
     invAll finalHeap finalRho finalAccess post
 .
 Proof.
   destruct s'';
-  do 7 intro;
+  do 6 intro;
   intro HO;
   intro INV;
   inversionx HO.
@@ -1105,8 +552,24 @@ Proof.
     set (fp := footprint initialHeap r' phi_pre).
     set (phi_pre' := phiType (xUserDef z) T_p :: phiType xthis (TClass C0) :: phi_pre) in *.
     set (phi_post' := phiType (xUserDef z) T_p :: phiType xthis (TClass C0) :: phiType xresult T_r :: phi_post) in *.
-    set (S'' := (initialRho, Aexcept initialAccess fp, sCall x0 x1 m0 x2 :: s') :: S').
+    set (S'' := [(initialRho, Aexcept initialAccess fp, sCall x0 x1 m0 x2 :: s')]).
     set (phi_end := phiSubsts3 xthis x1 (xUserDef z) x2 xresult x0 phi_post ++ phi_r).
+    
+    assert (r' xresult = Some (defaultValue T_r))
+    as r'xresult.
+      subst r'. unfold rhoFrom3. tauto.
+    
+    assert (r' xthis = Some (vo vo1))
+    as r'xthis.
+      subst r'. unfold rhoFrom3. tauto.
+    
+    assert (r' (xUserDef z) = Some v2)
+    as r'xUDz.
+      subst r'. unfold rhoFrom3.
+      dec (x_dec (xUserDef z) xresult). clear de2.
+      dec (x_dec (xUserDef z) xthis). clear de2.
+      dec (x_dec (xUserDef z) (xUserDef z)).
+      tauto.
     
     (*Part 1: make the call*)
     assert (evalphi initialHeap r' initialAccess phi_pre)
@@ -1118,19 +581,10 @@ Proof.
       eca; simpl.
         apply inclEmpty.
         eca; try apply hdtX2.
-        subst r'.
-        unfold rhoFrom3.
-        dec (x_dec (xUserDef z) xresult). clear de2.
-        dec (x_dec (xUserDef z) xthis). clear de2.
-        dec (x_dec (xUserDef z) (xUserDef z)).
-        eauto.
       common.
       eca; simpl.
         apply inclEmpty.
         eca; try apply hdtX1.
-        subst r'.
-        unfold rhoFrom3. simpl.
-        eauto.
       common.
       eapp evalphiFootprintAccess.
     
@@ -1139,10 +593,8 @@ Proof.
       eapp evalphiImpliesAccess.
     
     assert (dynSem 
-              (initialHeap, (initialRho, initialAccess, sCall x0 x1 m0 x2 :: s') 
-                            :: S')
-              (initialHeap, (r', fp, underscore) 
-                            :: S'')
+              (initialHeap, [(initialRho, initialAccess, sCall x0 x1 m0 x2 :: s')])
+              (initialHeap, (r', fp, underscore) :: S'')
            )
     as part1.
       eca; unfold evale; simpl. (*3*)
@@ -1174,24 +626,29 @@ Proof.
     (*Part 2: method body*)
     assert (∃ finalHeap finalRho finalAccess,
           dynSemStar 
-            (initialHeap, (r', fp, underscore) :: S'')
-            (finalHeap, (finalRho, finalAccess, []) :: S'') ∧
+            (initialHeap, [(r', fp, underscore)])
+            (finalHeap, [(finalRho, finalAccess, [])]) ∧
           invAll finalHeap finalRho finalAccess phi_post')
     as call_finished.
-      assert soundness as sdn. admit. (*assume that for method body*)
-      specialize (sdn phi_pre' underscore phi_post' initialHeap r' fp S'').
+      assert (soundness phi_pre' underscore phi_post' initialHeap r' fp []) as sdn. admit. (*assume that for method body*)
       intuition.
     
     invE call_finished finalHeap'.
     invE call_finished finalRho'.
     invE call_finished finalAccess'.
-    inversion call_finished as [part2 INV2]. clear call_finished.
+    inversion call_finished as [part2' INV2]. clear call_finished.
+    assert (dynSemStar 
+      (initialHeap, (r', fp, underscore) :: S'')
+      (finalHeap', (finalRho', finalAccess', []) :: S''))
+    as part2.
+      eapp (dynSemStarLift 
+             (initialHeap, [(r', fp, underscore)])
+             (finalHeap', [(finalRho', finalAccess', [])])).
     
     (*Part 3: call finished*)
     assert (exists vresult, finalRho' xresult = Some vresult)
     as vres.
       eapp RhoGetsMoreSpecific.
-      subst r'. unfold rhoFrom3. simpl. eauto.
     invE vres vresult.
     
     set (finalRho := rhoSubst x0 vresult initialRho).
@@ -1210,10 +667,8 @@ Proof.
     
     assert (dynSem
               (finalHeap', (finalRho', finalAccess', []) 
-                          :: (initialRho, Aexcept initialAccess fp , sCall x0 x1 m0 x2 :: s') 
-                          :: S')
-              (finalHeap',   (finalRho  , Aexcept initialAccess fp ++ footprint finalHeap' finalRho' phi_post, s') 
-                          :: S')
+                          :: [(initialRho, Aexcept initialAccess fp , sCall x0 x1 m0 x2 :: s')])
+              (finalHeap',   [(finalRho  , Aexcept initialAccess fp ++ footprint finalHeap' finalRho' phi_post, s')])
            )
     as part3.
       eapply HeapGetsMoreSpecific in part2; eauto. inversionE part2.
@@ -1225,6 +680,20 @@ Proof.
       (footprint finalHeap' finalRho (phiSubsts3 xthis x1 (xUserDef z) x2 xresult x0 phi_post))
       (Aexcept initialAccess fp ++ footprint finalHeap' finalRho' phi_post))
     as incl_FP_phi_post.
+      admit.
+    
+    assert (incl
+      (footprint finalHeap' finalRho (phiSubsts3 xthis x1 (xUserDef z) x2 xresult x0 phi_r))
+      (Aexcept
+        (Aexcept initialAccess fp ++ footprint finalHeap' finalRho' phi_post)
+        (footprint finalHeap' finalRho (phiSubsts3 xthis x1 (xUserDef z) x2 xresult x0 phi_post))))
+    as incl_FP_phi_r.
+      subst preI.
+      rewrite app_comm_cons in ep_preI.
+      apply evalphiApp in ep_preI.
+      inversionx ep_preI.
+      apply evalphiImpliesAccess in H1.
+      apply inclAexceptDisjoint in H1.
       admit.
     
     assert (evalphi
@@ -1246,23 +715,31 @@ Proof.
           apply mmwd.
           apply hdtX1.
           apply hdtX2.
+          eapply (dynSemStarNotModifies xthis _ _ _ r' finalRho') in part2'; eauto. apply mmwd.
+          eapply (dynSemStarNotModifies (xUserDef z) _ _ _ r' finalRho') in part2'; eauto. rewrite r'xUDz in *. rewrite part2'. tauto. apply mmwd.
+          simpl in xDist. intuition.
+          simpl in xDist. intuition.
+          simpl in xDist. intuition.
+    (**)subst preI.
+        rewrite app_comm_cons in ep_preI.
+        apply evalphiApp in ep_preI.
+        inversionx ep_preI.
+        
+        subst finalRho.
+        eapp evalphiRemoveRhoSubst.
+        
+        eapp evalphiIncl.
+        apply evalphiImpliesAccess in H1.
+        apply inclAexceptDisjoint in H1.
 
-Lemma dynSemStarNotModifies : forall x S ss H1 H2 r1 r2 A1 A2,
-  (∀ s', In s' ss → ¬ writesTo x s') ->
-  dynSemStar
-    (H1, (r1, A1, ss) :: S)
-    (H2, (r2, A2, []) :: S) ->
-  r1 x = r2 x.
-Proof.
-  induction ss; intros; simpl in *.
-  - inversionx H3; try tauto.
-
-          admit.
-          admit.
-          simpl in xDist. intuition.
-          simpl in xDist. intuition.
-          simpl in xDist. intuition.
-    (**)admit.
+Lemma 
+  dynSemStar (H1, [(r1, A1, s)]) (H2, [(r2, A2, [])]) ->
+  evale' H1 r1 o = evale H2 r1 o
+        
+Lemma 
+  evalphi H1 r A p ->
+  evalphi H2 r A p ->
+        
         
 
 (* Lemma InFootprintFV : forall
